src/solvers.v
@@ -37,3 +37,121 @@ Ltac solve_fAX tac1 init_l :=
 
 Ltac solve_fAnd tac1 tac2 init_ :=
 split; [> tac1 init_ | tac2 init_].
+
+
+Theorem usefull4: forall m n, S m = n -> m = n - 1.
+lia.
+Defined.
+Definition usefull: forall m n:nat, S m <= n -> S m = n \/ S m <= n - 1.
+lia.
+Defined. 
+
+Definition usefull2: forall m n:nat, S m = S n -> m = n .
+lia.
+Defined.
+Definition usefull3: forall m n:nat, m <= n -> m - 1 <= n - 1.
+lia.
+Defined. 
+Ltac solve_AU n max_of_state init_l solve_subformula1 solve_subformula2 := 
+let solve_AU max_of_state :=
+    let path_pi := fresh "path_pi" in
+    intro path_pi;
+    let is_path_pi := fresh "is_path_pi" in
+    intro is_path_pi;
+    let first_state:= fresh "first_state" in
+    intro first_state;
+    compute;
+    let (*rec*) sol_AU n :=
+    (* tryif (let h:= fresh "h" in assert(h: n <= max_of_state); [progress auto | auto])
+    then *)
+    (
+        eexists n (*n*); 
+        [
+            auto;
+            let m := fresh "m" in
+            let le_m := fresh "le_m" in
+            intro m;
+            intro le_m;
+            (
+            let rec solve_rec le_m := 
+                apply usefull in le_m; (*compute in le_m;*)
+                destruct le_m as [ le_m | le_m];
+                [>
+                (apply usefull2 in le_m) + lia (* for cases S m = 0*);
+                rewrite init_l in first_state;
+                try (rewrite <- le_m in first_state;
+                solve_subformula1 first_state);
+                let rec loop_to_needed_m i m :=
+                    tryif (let h:= fresh "h" in assert(h: i < m); [progress auto | auto])
+                    then 
+                        let is_path_pi_i := fresh "is_path_pi_i" in
+                        pose proof (is_path_pi i) as is_path_pi_i;
+                        compute in is_path_pi_i;
+                        repeat (
+                            let a := fresh "a" in
+                            let b := fresh "b" in
+                            destruct is_path_pi_i as (a&b);
+                            ((apply a in first_state)+(apply b in first_state));
+                            (
+                            lazymatch type of first_state with 
+                            | _ \/ _ => (repeat destruct first_state as [first_state|first_state])
+                            | _ => idtac
+                            end
+                            );
+                            loop_to_needed_m (i + 1) m)
+                    else 
+                        idtac
+                in
+                lazymatch type of le_m with 
+                | _ = ?k => loop_to_needed_m 0 k
+                | _ => idtac
+                end
+                ;
+                rewrite <- le_m in first_state;
+                solve_subformula1 first_state
+                
+                |
+                (compute in le_m;
+                lia) +  
+                (solve_rec le_m) + auto
+                ]
+            in
+            (solve_rec le_m)
+            )
+            
+        |
+        auto;
+        rewrite init_l in first_state;
+        let rec loop_to_needed_m i m :=
+            tryif (let h:= fresh "h" in assert(h: i < m); [progress auto | auto])
+            then 
+                let is_path_pi_i := fresh "is_path_pi_i" in
+                pose proof (is_path_pi i) as is_path_pi_i;
+                compute in is_path_pi_i;
+                repeat (
+                    let a := fresh "a" in
+                    let b := fresh "b" in
+                    destruct is_path_pi_i as (a&b);
+                    ((apply a in first_state)+(apply b in first_state));
+                    (repeat (
+                    lazymatch type of first_state with 
+                    | _ \/ _ => (destruct first_state as [first_state|first_state])
+                    | _ => idtac
+                    end
+                    ));
+                    loop_to_needed_m (i + 1) m)
+            else 
+                idtac
+        in
+        loop_to_needed_m 0 n;
+        solve_subformula2 first_state
+        ]
+    )
+    (* +
+    sol_AU (n + 1)
+    else 
+    fail "solve_AU: with" n*)
+    in 
+    sol_AU n
+in
+solve_AU max_of_state .
